cleaning st2 a bit

lib/st2.fst
@@ -7,47 +7,16 @@ module Comp
 open Heap
 type heap2 = heap * heap
 
-(* Working around https://github.com/FStarLang/FStar/issues/164 *)
-kind STWP (a:Type) = (a -> heap -> Type) -> heap -> Type
-kind PUREWP (a:Type) = (a -> Type) -> Type
-kind ALLPost (a:Type) = result a -> heap -> Type
-
-monad_lattice {
-  STATE2:: (* STATE a wp wlp *)
-          kind Pre     = heap2 -> Type
-          kind Post (a:Type) = a -> heap2 -> Type
-          kind WP (a:Type) = Post a -> Pre
-          type return   (a:Type) (x:a) (p:Post a) = p x
-          type bind_wp  (a:Type) (b:Type) (wp1:WP a) (wlp1:WP a) (wp2:(a -> WP b)) (wlp2:(a -> WP b)) (p:Post b) (h0:heap2) =
-              wp1 (fun a h1 -> wp2 a p h1) h0
-          type bind_wlp (a:Type) (b:Type) (wlp1:WP a) (wlp2:(a -> WP b)) (p:Post b) (h0:heap2) = wlp1 (fun a -> wlp2 a p) h0
-          type if_then_else (a:Type) (p:Type) (wp_then:WP a) (wp_else:WP a) (post:Post a) (h0:heap2) =
-              (if p
-               then wp_then post h0
-               else wp_else post h0)
-          type ite_wlp  (a:Type) (wlp_cases:WP a) (post:Post a) (h0:heap2) =
-              (forall (a:a) (h:heap2). wlp_cases (fun a1 h1 -> a=!=a1 \/ h=!=h1) h0 \/ post a h)
-          type ite_wp (a:Type) (wlp_cases:WP a) (wp_cases:WP a) (post:Post a) (h0:heap2) =
-              (forall (a:a) (h:heap2). wlp_cases (fun a1 h1 -> a=!=a1 \/ h=!=h1) h0 \/ post a h)
-              /\ wp_cases (fun a h_ -> True) h0
-          type wp_binop (a:Type) (wp1:WP a) ('op:Type -> Type -> Type) (wp2:WP a) (p:Post a) (h:heap2) =
-              'op (wp1 p h) (wp2 p h)
-          type wp_as_type (a:Type) (wp:WP a) = (forall (p:Post a) (h:heap2). wp p h)
-          type close_wp (a:Type) (b:Type) (wp:(b -> WP a)) (p:Post a) (h:heap2) = (forall (b:b). wp b p h)
-          type close_wp_t (a:Type) (wp:(Type -> WP a)) (p:Post a) (h:heap2) = (forall (b:Type). wp b p h)
-          type assert_p (a:Type) ('P:Type) (wp:WP a) (p:Post a) (h:heap2) = ('P /\ wp p h)
-          type assume_p (a:Type) ('P:Type) (wp:WP a) (p:Post a) (h:heap2) = ('P ==> wp p h)
-          type null_wp (a:Type) (p:Post a) (h:heap2) = (forall (x:a) (h':heap2). p x h')
-          type trivial (a:Type) (wp:WP a) = (forall h0. wp (fun r h1 -> True) h0)
-          with ST2 (a:Type) (pre:Pre) (post: (heap2 -> Post a)) =
-              STATE2 a
-                (fun (p:Post a) (h:heap2) -> pre h /\ (forall a h1. (pre h /\ post h a h1) ==> p a h1)) (* WP *)
-                (fun (p:Post a) (h:heap2) -> (forall a h1. (pre h /\ post h a h1) ==> p a h1))           (* WLP *)
-          and St2 (a:Type) = ST2 a (fun h -> True) (fun h0 r h1 -> True)
-  with
-  PURE   ~> STATE2 = (fun ('a:Type) ('wp:PUREWP 'a) ('p:STATE2.Post 'a) -> (fun h2 -> 'wp (fun a0 -> 'p a0 h2)));
-  STATE2 ~> ALL    = (fun ('a:Type) ('wp:STATE2.WP 'a) ('p:ALLPost 'a) -> (fun h -> False))
-}
+new_effect STATE2 = STATE_h heap2
+kind ST2Pre = STPre_h heap2
+kind ST2Post (a:Type) = STPost_h heap2 a
+effect ST2 (a:Type) (pre:ST2Pre) (post: (heap2 -> ST2Post a)) =
+    STATE2 a
+      (fun (p:STPost_h heap2 a) (h:heap2) -> pre h /\ (forall a h1. (pre h /\ post h a h1) ==> p a h1)) (* WP *)
+      (fun (p:STPost_h heap2 a) (h:heap2) -> (forall a h1. (pre h /\ post h a h1) ==> p a h1))           (* WLP *)
+effect St2 (a:Type) = ST2 a (fun h -> True) (fun h0 r h1 -> True)
+sub_effect
+  PURE   ~> STATE2 = (fun (a:Type) (wp:PureWP a) (p:ST2Post a) -> (fun h2 -> wp (fun a0 -> p a0 h2)))
 
 type comp (a:Type) (b:Type) (wp0:STWP a) (wp1:STWP b) (p:((a * b) -> heap2 -> Type)) (h2:heap2) =
     wp0 (fun y0 h0 ->
@@ -65,11 +34,14 @@ assume val compose2: a0:Type -> b0:Type -> wp0:(a0 -> STWP b0) -> wlp0:(a0 -> ST
                              (comp b0 b1 (wp0 x0) (wp1 x1))
                              (comp b0 b1 (wlp0 x0) (wlp1 x1))
 
+module Samples
+open Comp
+open Heap
 let f x = x := !x - !x
 let g x = x := 0
 val equiv1: x:ref int
          -> y:ref int
-         -> STATE2.ST2 (unit * unit)
+         -> ST2 (unit * unit)
                 (requires (fun _ -> True)) //x, y may be high-references
                 (ensures (fun _ _ h2' -> sel (fst h2') x == sel (snd h2') y)) //their contents are equal afterwards
 let equiv1 x y = compose2 f g x y
@@ -78,7 +50,7 @@ let equiv1 x y = compose2 f g x y
 let square x = x := !x * !x
 val equiv2: x:ref int
          -> y:ref int
-         -> STATE2.ST2 (unit * unit)
+         -> Comp.ST2 (unit * unit)
                 (requires (fun h2 -> sel (fst h2) x = - (sel (snd h2) y)))     //x, y negatives of each other
                 (ensures (fun _ _ h2' -> sel (fst h2') x = sel (snd h2') y)) //their contents are equal afterwards
 let equiv2 x y = compose2 square square x y
@@ -88,7 +60,7 @@ let f3 x = if !x = 0 then x := 0 else x:= 1
 let g3 x = if !x <> 0 then x := 1 else x:= 0
 val equiv3: x:ref int
          -> y:ref int
-         -> STATE2.ST2 (unit * unit)
+         -> Comp.ST2 (unit * unit)
                 (requires (fun h -> sel (fst h) x = sel (snd h) y)) // x, y have same values
                 (ensures (fun _ _ h2' -> sel (fst h2') x = sel (snd h2') y)) // their contents are equal afterwards
 let equiv3 x y = compose2 f3 g3 x y
@@ -98,7 +70,7 @@ let f4 x = if !x = 0 then x := 0 else x:= 1
 let g4 x = if !x = 0 then x := 1 else x:= 0
 val equiv4: x:ref int
          -> y:ref int
-         -> STATE2.ST2 (unit * unit)
+         -> Comp.ST2 (unit * unit)
                 (requires (fun h -> if sel (fst h) x = 0 then sel (snd h) y = 1 else sel (snd h) y = 0)) // making sure !x=0 <==> !y <> 0
                 (ensures (fun _ _ h2' -> sel (fst h2') x = sel (snd h2') y)) //their contents are equal afterwards
 let equiv4 x y = compose2 f4 g4 x y
@@ -108,7 +80,7 @@ let f5 x = x := 0
 let g5 x = if !x = 0 then x := !x else x:= !x - !x
 val equiv5: x:ref int
          -> y:ref int
-         -> STATE2.ST2 (unit * unit)
+         -> Comp.ST2 (unit * unit)
                 (requires (fun _ -> True))  // no requirements
                 (ensures (fun _ _ h2' -> sel (fst h2') x = sel (snd h2') y)) //their contents are equal afterwards
 let equiv5 x y = compose2 f5 g5 x y
@@ -118,7 +90,7 @@ let f6 x = let y = 1 in x := y
 let g6 x = if !x = 0 then x := 1 else if !x <> 0 then x := 1 else x:= 0
 val equiv6: x:ref int
          -> y:ref int
-         -> STATE2.ST2 (unit * unit)
+         -> Comp.ST2 (unit * unit)
                 (requires (fun _ -> True)) // no requirements
                 (ensures (fun _ _ h2' -> sel (fst h2') x = sel (snd h2') y)) //their contents are equal afterwards
 let equiv6 x y = compose2 f6 g6 x y
@@ -128,7 +100,7 @@ let f7 x = x := 2*!x
 let g7 x = let y = (fun a -> a + a) !x in x := y
 val equiv7: x:ref int
          -> y:ref int
-         -> STATE2.ST2 (unit * unit)
+         -> Comp.ST2 (unit * unit)
                 (requires (fun h -> sel (fst h) x - sel (snd h) y = 10)) // values of x, y differ by 10
                 (ensures (fun _ _ h2' -> sel (fst h2') x - sel (snd h2') y = 20)) // values of x, y differ by 20
 let equiv7 x y = compose2 f7 g7 x y
@@ -137,7 +109,7 @@ let equiv7 x y = compose2 f7 g7 x y
 let f8 (x, y, z) = if !z=0 then (x := 1; y := 1) else (y:=1 ; x := 0)
 val equiv8: a:(ref int * ref int * ref int)
          -> b:(ref int * ref int * ref int)
-         -> STATE2.ST2 (unit * unit)
+         -> Comp.ST2 (unit * unit)
                 (requires (fun h -> MkTuple3._1 a <> MkTuple3._2 a /\  // x and y are not aliases
                                     MkTuple3._1 b <> MkTuple3._2 b))
                 (ensures (fun _ _ h2' -> sel (fst h2') (MkTuple3._2 a) = sel (snd h2') (MkTuple3._2 b))) //value of y is the same
@@ -151,7 +123,7 @@ let equiv8 a b = compose2 f8 f8 a b
 let assign x y = x := y
 
 val monotonic_assign : x:ref int -> y1:int -> y2:int
-                       -> STATE2.ST2 (unit * unit)
+                       -> Comp.ST2 (unit * unit)
                                      (requires (fun h -> y1 <= y2))
                                      (ensures (fun h1 r h2 -> sel (fst h2) x <= sel (snd h2) x))
 let monotonic_assign x y1 y2 = compose2 (assign x) (assign x) y1 y2
@@ -167,7 +139,7 @@ let monotonic_id_standard x y = ()
 
 
 (* This does not work...? *)
-(* val monotonic_id : x:int -> y:int -> STATE2.ST2 (int * int) *)
+(* val monotonic_id : x:int -> y:int -> Comp.ST2 (int * int) *)
 (*                                                 (requires (fun h -> x <= y)) *)
 (*                                                 (ensures (fun h1 r h2 -> (fst r) <= (snd r))) *)
 (* let monotonic_id x y = compose2 id id x y *)
@@ -229,7 +201,7 @@ val noleak_ok: x1:ref int
                -> x2:ref int
                -> b1:bool
                -> b2:bool
-               -> STATE2.ST2 (unit * unit)
+               -> Comp.ST2 (unit * unit)
                              (requires (fun h -> True))
                              (ensures (fun h1 r h2 -> ((x1 = x2) /\ (fst h1 = snd h1)) ==> (fst h2 = snd h2)))
 let noleak_ok x1 x2 b1 b2 = compose2 noleak noleak (x1,b1) (x2,b2)
